\begin{frame}[fragile]
\frametitle{Mappable}
\framesubtitle{The interface}
\begin{block}{Java 8 with higher-kinds}
\begin{lstlisting}[style=language,language=java]
interface Mappable<T> {
  <A, B> T<B> map(Function<A, B> f, T<A> a);
}
\end{lstlisting}
\end{block}
\begin{block}{Haskell}
\begin{lstlisting}[style=language,language=haskell]
class Mappable t where
  map :: (a -> b) -> t a -> t b
\end{lstlisting}
\end{block}
\end{frame}

\begin{frame}[fragile]
\frametitle{Mappable}
\framesubtitle{The laws}
\begin{block}{Identity}
\begin{lstlisting}[style=language,language=haskell]
map (\z -> z) x == x
\end{lstlisting}
\end{block}
\begin{block}{Composition}
\begin{lstlisting}[style=language,language=haskell]
map (\z -> f (g z)) x == map f (map g x)
\end{lstlisting}
\end{block}
\end{frame}

\begin{frame}[fragile]
\frametitle{Mappable}
\framesubtitle{The instances}
\begin{block}{List \lstinline{[]}}
\begin{lstlisting}[style=language,language=haskell]
map :: (a -> b) -> [a] -> [b]
map f x = foldr ((:) . f) [] x
\end{lstlisting}
\end{block}
\begin{block}{Reader \lstinline{((->) e)}}
\begin{lstlisting}[style=language,language=haskell]
map :: (a -> b) -> (e -> a) -> (e -> b)
map f g = \e -> f (g e)
\end{lstlisting}
\end{block}
\end{frame}

\begin{frame}[fragile]
\frametitle{Mappable}
\framesubtitle{The derived operations}
\begin{block}{Map a constant value}
\begin{lstlisting}[style=language,language=haskell]
mapConstant :: Mappable f => a -> t b -> t a
mapConstant a b = fmap (\_ -> a) b
\end{lstlisting}
\end{block}
\begin{block}{Reader \lstinline{((->) e)}}
\begin{lstlisting}[style=language,language=haskell]
mapApply :: t (a -> b) -> a -> t b
mapApply f a = fmap (\g -> g a) f

\end{lstlisting}
\end{block}
\end{frame}
